\documentclass[12pt]{extarticle}
%Some packages I commonly use.
\usepackage[english]{babel}
\usepackage{graphicx}
\usepackage{framed}
\usepackage[normalem]{ulem}
\usepackage{amsmath}
\usepackage{amsthm}
\usepackage{amssymb}
\usepackage{amsfonts}
\usepackage{enumerate}
\usepackage[utf8]{inputenc}
\usepackage[top=1 in,bottom=1in, left=1 in, right=1 in]{geometry}

%A bunch of definitions that make my life easier
\newcommand{\matlab}{{\sc Matlab} }
\newcommand{\abs}[1]{|#1|}
\newcommand{\set}[1]{\{#1\}}
\newcommand{\cvec}[1]{{\mathbf #1}}
\newcommand{\rvec}[1]{\vec{\mathbf #1}}
\newcommand{\ihat}{\hat{\textbf{\i}}}
\newcommand{\jhat}{\hat{\textbf{\j}}}
\newcommand{\khat}{\hat{\textbf{k}}}
\newcommand{\minor}{{\rm minor}}
\newcommand{\trace}{{\rm trace}}
\newcommand{\spn}{{\rm Span}}
\newcommand{\rem}{{\rm rem}}
\newcommand{\ran}{{\rm range}}
\newcommand{\range}{{\rm range}}
\newcommand{\mdiv}{{\rm div}}
\newcommand{\proj}{{\rm proj}}
\newcommand{\R}{\mathbb{R}}
\newcommand{\N}{\mathbb{N}}
\newcommand{\Q}{\mathbb{Q}}
\newcommand{\Z}{\mathbb{Z}}
\newcommand{\<}{\langle}
\renewcommand{\>}{\rangle}
\renewcommand{\emptyset}{\varnothing}
\newcommand{\attn}[1]{\textbf{#1}}
\theoremstyle{definition}
\newtheorem{theorem}{Theorem}
\newtheorem{prob}{Problem}
\newtheorem{corollary}{Corollary}
\newtheorem*{definition}{Definition}
\newtheorem*{example}{Example}
\newtheorem*{note}{Note}
\newtheorem{exercise}{Exercise}
\newcommand{\bproof}{\bigskip {\bf Proof. }}
\newcommand{\eproof}{\hfill\qedsymbol}
\newcommand{\Disp}{\displaystyle}
\newcommand{\qe}{\hfill\(\bigtriangledown\)}
\setlength{\columnseprule}{1 pt}


\title{ Math 5205 -- Topology Assignment 3}
\author{David Draguta}
\date{2021-10-18}

\begin{document}

\maketitle

\begin{exercise}
  Let $(X_{\alpha})_{\alpha \in A}$ be a non-empty family of topological spaces and $\varphi: A \to A$ a bijection of $A$ onto $A$. Prove that the cartesian product
  $\prod\limits_{\alpha \in A}X_{\alpha}$ and $\prod\limits_{\alpha \in A}X_{\varphi{\alpha}}$ are homeomorphic. 
\end{exercise}
\begin{proof}
  We define $f: \prod\limits_{\alpha \in A}X_{\alpha} \to \prod\limits_{\alpha \in A}X_{\varphi(\alpha)}$ by $ f(x) = x \circ \varphi$ and $g: f: \prod\limits_{\alpha \in A}X_{\varphi(\alpha)} \to \prod\limits_{\alpha \in A}X_{\alpha}$ by $g(x') = x' \circ \varphi^{-1}$, and check that these are continuous inverses of each other. We first check that the two are inverses of each other (which shows they're bijections)
  \begin{align*}
    g(f(x))  &= g(x \circ \varphi)     = (x \circ \varphi) \circ \varphi^{-1} = x \circ (\varphi \circ \varphi^{-1}) \\
    &= x, 
  \end{align*}
  and
  \begin{align*}
    f(g(x')) &= f(x'\circ \varphi^{-1}) = (x' \circ \varphi^{-1}) \circ \varphi = x' \circ (\varphi^{-1} \circ \varphi) \\
    &= x'.
  \end{align*}
  Next, we use Thm 101 part 3 to show that $f,g$ are continuous. For each $\alpha \in A$ and $(x_{\alpha})_{\alpha \in A} \in \prod\limits_{\alpha \in A}X_{\alpha}$ we have 
  \begin{align*}
    (\pi_\alpha \circ f)((x_{\alpha})_{\alpha \in A}) &= \pi_\alpha(f((x_{\alpha})_{\alpha \in A})) = \pi_{\alpha}((x_{\alpha})_{\alpha \in A} \circ \varphi) = \pi_{\alpha}((x_{\varphi(\alpha)})_{\alpha \in A}) = x_{\varphi(\alpha)} \\
    &= \pi_{\varphi(\alpha)}(x_{\alpha}_{\alpha \in A}),
  \end{align*}
  and so
  \begin{align*}
    \pi_{\alpha} \circ f  = \pi_{\varphi(\alpha)}.
  \end{align*}
  is continous for all $\alpha \in A$. We conclude that $f$ is continuous (with respect to the weak topology).

  Similarly for $\alpha \in A$ and $(x_{\varphi(\alpha)})_{\alpha \in A} \in \prod\limits_{\alpha \in A} X_{\varphi(\alpha)}$, we have
  \begin{align*}
    (\pi_{\alpha}\circ g)((x_{\varphi(\alpha)})_{\alpha \in A}) &= \pi_{\alpha}(g((x_{\varphi(\alpha)})_{\alpha \in A})) = \pi_{\alpha}((x_{\varphi(\alpha)})_{\alpha \in A} \circ \varphi^{-1}) = \pi_{\alpha}((x_{\alpha})_{\alpha \in A}) = x_{\alpha} \\
    &= \pi_{\varphi^{-1}(\alpha)}((x_{\varphi(\alpha)})_{\alpha \in A}),
  \end{align*}
  so
  \begin{align*}
    \pi_{\alpha}\circ g = \pi_{\varphi^{-1}(\alpha)}.
  \end{align*}
\end{proof}
\end{document}



